LeanSorting/Nat/Extras.lean
@@ -1,0 +1,4 @@
+import Mathlib.Data.Nat.Defs
+
+def Nat.in_range (n : ℕ) (low high : ℕ) : Prop := n ≥ low ∧ n < high
+def Nat.adjacent_in_range (n m low high : ℕ) : Prop := n.succ = m ∧ n ≥ low ∧ m < high
